========
Tutorial
========

This is a tutorial on Elastic net Regularized Generalized Linear Models.
We will go through the math and gradient descent algorithm to
in order to optimize GLM cost function.

**Reference**
Jerome Friedman, Trevor Hastie and Rob Tibshirani. (2010).
Regularization Paths for Generalized Linear Models via Coordinate Descent.
Journal of Statistical Software, Vol. 33(1), 1-22 `[pdf]
<https://core.ac.uk/download/files/153/6287975.pdf>`_.


.. code-block:: python

   # Author: Pavan Ramkumar
   # License: MIT

   import numpy as np
   from scipy.special import expit



GLM with elastic net penalty
----------------------------

In Generalized Linear Model (GLM), we mainly want to solve the following problem.

.. math::

    \min_{\beta_0, \beta} \frac{1}{N} \sum_{i = 1}^N w_i \ell (y_i, \beta_0 + \beta^T x_i)
    + \lambda [0.5(1 - \alpha)\| \beta \|_2^2 + \alpha \| \beta \|_1]

where :math:`\ell (y_i, \beta_0 + \beta^T x_i)` is negative log-likelihood of
an observation :math:`i`. Here, we will go through Poisson link function case
and show how we can optimize this cost function

Poisson-like GLM
----------------
The `pyglmnet` implementation comes with `poisson`, `binomial`
and `normal` distributions, but for illustration, we will walk you
through a particular adaptation of the canonical Poisson generalized
linear model (GLM).

For the Poisson GLM, :math:`\lambda_i` is the rate parameter of an
inhomogeneous linear-nonlinear Poisson (LNP) process with instantaneous
mean given by:

.. math::   \lambda_i = \exp(\beta_0 + \beta^T x_i)

where :math:`x_i \in \mathcal{R}^{p \times 1}, i = \{1, 2, \dots, n\}` are
the observed independent variables (predictors),
:math:`\beta_0 \in \mathcal{R}^{1 \times 1}`,
:math:`\beta \in \mathcal{R}^{p \times 1}`
are linear coefficients. :math:`\lambda_i` is also known as the conditional
intensity function, conditioned on :math:`(\beta_0, \beta)` and
:math:`q(z) = \exp(z)` is the nonlinearity.

For numerical reasons, let's adopt a stabilizing non-linearity, known as the
softplus or the smooth rectifier `Dugas et al., 2001
<http://papers.nips.cc/paper/1920-incorporating-second-order-functional-knowledge-for-better-option-pricing.pdf>`_,
and adopted by Jonathan Pillow's and Liam Paninski's groups for neural data
analysis.
See for instance: `Park et al., 2014
<http://www.nature.com/neuro/journal/v17/n10/abs/nn.3800.html>`_.

.. math::    q(z) = \log(1+\exp(z))

The softplus prevents :math:`\lambda` in the canonical inverse link function
from exploding when the argument to the exponent is large. In this
modification, the formulation is no longer an exact LNP, nor an exact GLM,
but :math:\pm\mathcal{L}(\beta_0, \beta)` is still concave (convex) and we
can use gradient ascent (descent) to optimize it.

.. math::    \lambda_i = q(\beta_0 + \beta^T x_i) = \log(1 + \exp(\beta_0 +
                           \beta^T x_i))

[There is more to be said about this issue; ref. Sara Solla's GLM lectures
concerning moment generating functions and strict definitions of GLMs]\

.. code-block:: python

   def qu(z):
      """The non-linearity."""
      qu = np.log1p(np.exp(z))

   def lmb(self, beta0, beta, X):
      """Conditional intensity function."""
      z = beta0 + np.dot(X, beta)
      l = self.qu(z)
      return l


Poisson Log-likelihood
----------------------
The likelihood of observing the spike count :math:`y_i` under the Poisson
likelihood function with inhomogeneous rate :math:`\lambda_i` is given by:

.. math::    \prod_i P(y = y_i) = \prod_i \frac{e^{-\lambda_i} \lambda_i^{y_i}}{y_i!}

The log-likelihood is given by:

.. math::    \mathcal{L} = \sum_i \bigg\{y_i \log(\lambda_i) - \lambda_i
                           - log(y_i!)\bigg\}

However, we are interested in maximizing the log-likelihood as a function of
:math:`\beta_0` and :math:`\beta`. Thus, we can drop the factorial term:

.. math::    \mathcal{L}(\beta_0, \beta) = \sum_i \bigg\{y_i \log(\lambda_i)
                                          - \lambda_i\bigg\}

Elastic net penalty
-------------------
For large models we need to penalize the log likelihood term in order to
prevent overfitting. The elastic net penalty is given by:

.. math::    \mathcal{P}_\alpha(\beta) = (1-\alpha)\frac{1}{2} \|\beta\|^2_{\mathcal{l}_2} + \alpha\|\beta\|_{\mathcal{l}_1}

The elastic net interpolates between two extremes.
:math:`\alpha = 0` is known as ridge regression and :math:`\alpha = 1`
is known as LASSO. Note that we do not penalize the baseline term
:math:`\beta_0`.


.. code-block:: python

   def penalty(alpha, beta):
      """the penalty term"""
      P = 0.5 * (1 - alpha) * np.linalg.norm(beta, 2) + \
            alpha * np.linalg.norm(beta, 1)
      return P

Objective function
------------------

We minimize the objective function:

.. math::

     J(\beta_0, \beta) = -\mathcal{L}(\beta_0, \beta) + \lambda \mathcal{P}_\alpha(\beta)

where :math:`\mathcal{L}(\beta_0, \beta)` is the Poisson log-likelihood and
:math:`\mathcal{P}_\alpha(\beta)` is the elastic net penalty term and
:math:`\lambda` and :math:`\alpha` are regularization parameters.

.. code-block:: python

   def loss(beta0, beta, reg_lambda, X, y):
      """Define the objective function for elastic net."""
      L = logL(beta0, beta, X, y)
      P = penalty(beta)
      J = -L + reg_lambda * P
         return J


Gradients descent
-----------------

To calculate the gradients of the cost function with respect to :math:`\beta_0` and
:math:`\beta`, let's plug in the definitions for the log likelihood and penalty terms from above.

.. math::

     \begin{eqnarray}
         J(\beta_0, \beta) &= \sum_i \bigg\{ \log(1 + \exp(\beta_0 + \beta^T x_i))\\
           & - y_i \log(\log(1 + \exp(\beta_0 + \beta^T x_i)))\bigg\}\\
           & + \lambda(1 - \alpha)\frac{1}{2} \|\beta\|^2_{\mathcal{l_2}}
           + \lambda\alpha\|\beta\|_{\mathcal{l_1}}
     \end{eqnarray}


Since we will apply co-ordinate descent, let's rewrite this cost in terms of each
scalar parameter :math:`\beta_j`

.. math::

     \begin{eqnarray}
         J(\beta_0, \beta) &= \sum_i \bigg\{ \log(1 + \exp(\beta_0 + \sum_j \beta_j x_{ij}))
         & - y_i \log(\log(1 + \exp(\beta_0 + \sum_j \beta_j x_{ij})))\bigg\}\\
         & + \lambda(1-\alpha)\frac{1}{2} \sum_j \beta_j^2 + \lambda\alpha\sum_j \mid\beta_j\mid
     \end{eqnarray}

Let's take the derivatives of some big expressions using chain rule.
Define :math:`z_i = \beta_0 + \sum_j \beta_j x_{ij}`.

For the nonlinearity in the first term :math:`y = q(z) = \log(1+e^{z(\theta)})`,

.. math::

     \begin{eqnarray}
     \frac{\partial y}{\partial \theta} &= \frac{\partial q}{\partial z}\frac{\partial z}{\partial \theta}\\
     & = \frac{e^z}{1+e^z}\frac{\partial z}{\partial \theta}\\
     & = \sigma(z)\frac{\partial z}{\partial \theta}
     \end{eqnarray}

For the nonlinearity in the second term :math:`y = \log(q(z)) = \log(\log(1+e^{z(\theta)}))`,

.. math::

     \begin{eqnarray}
     \frac{\partial y}{\partial \theta} & = \frac{1}{q(z)}\frac{\partial q}{\partial z}\frac{\partial z}{\partial \theta}\\
     & = \frac{\sigma(z)}{q(z)}\frac{\partial z}{\partial \theta}
     \end{eqnarray}

where :math:`\dot q(z)` happens to be be the sigmoid function,

.. math::

     \sigma(z) = \frac{e^z}{1+e^z}

Putting it all together, we have,

.. math::

     \frac{\partial J}{\partial \beta_0} = \sum_i \sigma(z_i) - \sum_i y_i\frac{\sigma(z_i)}{q(z_i)}

.. math::

     \frac{\partial J}{\partial \beta_j} = \sum_i \sigma(z_i) x_{ij} - \sum_i y_i \frac{\sigma(z_i)}{q(z_i)}x_{ij}
     + \lambda(1-\alpha)\beta_j + \lambda\alpha \text{sgn}(\beta_j)

Let's define these gradients

.. code-block:: python

   def grad_L2loss(beta0, beta, reg_lambda, X, y):
      z = beta0 + np.dot(X, beta)
      s = expit(z)
      q = qu(z)
      grad_beta0 = np.sum(s) - np.sum(y * s / q)
        grad_beta = np.transpose(np.dot(np.transpose(s), X) -
                    np.dot(np.transpose(y * s / q), X)) + \
        reg_lambda * (1 - alpha) * beta
        return grad_beta0, grad_beta


Note that this is all we need for a classic batch gradient descent implementation.
However, let's also derive the Hessian terms that will be useful for second-order
optimization methods.

Hessian terms
-------------

Second-order derivatives can accelerate convergence to local minima by providing
optimal step sizes. However, they are expensive to compute.

This is where co-ordinate descent shines. Since we update only one parameter
:math:`\beta_j` per step, we can simply use the :math:`j^{th}` diagonal term in
the Hessian matrix to perform an approximate Newton update as:

.. math::

     \beta_j^{t+1} = \beta_j^{t} - \bigg\{\frac{\partial^2 J}{\partial \beta_j^2}\bigg\}^{-1} \frac{\partial J}{\partial \beta_j}

Let's use calculus again to compute these diagonal terms. Recall that:

.. math::

     \begin{eqnarray}
     \dot q(z) & = \sigma(z)\\
     \dot\sigma(z) = \sigma(z)(1-\sigma(z))
     \end{eqnarray}

Using these, and applying the product rule

.. math::

    \frac{\partial}{\partial z}\bigg\{ \frac{\sigma(z)}{q(z)} \bigg\} = \frac{\sigma(z)(1-\sigma(z))}{q(z)} - \frac{\sigma(z)}{q(z)^2}

Plugging all these in, we get

.. math::
     \frac{\partial^2 J}{\partial \beta_0^2} = \sum_i \sigma(z_i)(1 - \sigma(z_i)) - \sum_i y_i \bigg\{ \frac{\sigma(z_i) (1 - \sigma(z_i))}{q(z_i)} - \frac{\sigma(z_i)}{q(z_i)^2} \bigg\}

.. math::

     \begin{eqnarray}
     \frac{\partial^2 J}{\partial \beta_j^2} & = \sum_i \sigma(z_i)(1 - \sigma(z_i)) x_{ij}^2 \\
     & - \sum_i y_i \bigg\{ \frac{\sigma(z_i) (1 - \sigma(z_i))}{q(z_i)} \\
     & - \frac{\sigma(z_i)}{q(z_i)^2} \bigg\}x_{ij}^2 + \lambda(1-\alpha)
     \end{eqnarray}


.. code-block:: python

    def hessian_loss(beta0, beta, alpha, reg_lambda, X, y):
        z = beta0 + np.dot(X, beta)
        q = qu(z)
        s = expit(z)
        grad_s = s * (1-s)
        grad_s_by_q = grad_s/q - s/(q * q)
        hess_beta0 = np.sum(grad_s) - np.sum(y * grad_s_by_q)
        hess_beta = np.transpose(np.dot(np.transpose(grad_s), X * X)
                    - np.dot(np.transpose(y * grad_s_by_q), X * X))\
                    + reg_lambda * (1-alpha)
        return hess_beta0, hess_beta

Cyclical co-ordinate descent
----------------------------

**Parameter update step**

In cylical coordinate descent with elastic net, we store an active set,
:math:`\mathcal{K}`, of parameter indices that we update. Since the :math:`\mathcal{l}_1`
terms :math:`|\beta_j|` are not differentiable at zero, we use the gradient without
the :math:`\lambda\alpha \text{sgn}(\beta_j)` term to update :math:`\beta_j`.
Let's call these gradient terms :math:`\tilde{g}_k`.

We start by initializing :math:`\mathcal{K}` to contain all parameter indices
Let's say only the :math:`k^{th}` parameter is updated at time step :math:`t`.

.. math::

     \begin{eqnarray}
         \beta_k^{t} & = \beta_k^{t-1} - (h_k^{t-1})^{-1} \tilde{g}_k^{t-1} \\
         \beta_j^{t} & = \beta_j^{t-1}, \forall j \neq k
     \end{eqnarray}


Next, we apply a soft thresholding step for :math:`k \neq 0` after every update iteration, as follows.
:math:`\beta_k^{t} = \mathcal{S}_{\lambda\alpha}(\beta_k^{t})`

where

.. math::

     S_\lambda(x) =
     \begin{cases}
     0 & \text{if} & |x| \leq \lambda\\
     \text{sgn}(x)||x|-\lambda| & \text{if} & |x| > \lambda
     \end{cases}

If :math:`\beta_k^{t}` has been zero-ed out, we remove :math:`k` from the active set.

.. math::

     \mathcal{K} = \mathcal{K} \setminus \left\{k\right\}


.. code-block:: python

    def prox(X, l):
        """Proximal operator."""
        return np.sign(X) * (np.abs(X) - l) * (np.abs(X) > l)


**Efficient z update**

Next, we want to update :math:`\beta_{k+1}` at the next time step :math:`t+1`.
For this we need the gradient and Hessian terms, :math:`\tilde{g}_{k+1}` and
:math`h_{k+1}`. If we update them instead of recalculating them, we can save on
a lot of multiplications and additions. This is possible because we only update
one parameter at a time. Let's calculate how to make these updates.

.. math::

    z_i^{t} = z_i^{t-1} - \beta_k^{t-1}x_{ik} + \beta_k^{t}x_{ik}

.. math::

    z_i^{t} = z_i^{t-1} - (h_k^{t-1})^{-1} \tilde{g}_k^{t-1}x_{ik}


**Gradient update**

If :math:`k = 0`,

.. math::

     \tilde{g}_{k+1}^t = \sum_i \sigma(z_i^t) - \sum_i y_i \frac{\sigma(z_i^t)}{q(z_i^t)}

If :math:`k > 0`,

.. math::

     \begin{eqnarray}
         \tilde{g}_{k+1}^t & = \sum_i \sigma(z_i^t) x_{i,k+1} - \sum_i y_i \frac{\sigma(z_i^t)}{q(z_i^t)} x_{i,k+1}
           & + \lambda(1-\alpha)\beta_{k+1}^t
     \end{eqnarray}

.. code-block:: python

    def grad_loss_k(z, beta_k, alpha, rl, xk, y, k):
        """Gradient update for a single coordinate
        """
        q = qu(z)
        s = expit(z)
        if(k == 0):
            gk = np.sum(s) - np.sum(y*s/q)
        else:
            gk = np.sum(s*xk) - np.sum(y*s/q*xk) + rl*(1-alpha)*beta_k
        return gk


**Hessian update**

If :math:`k = 0`,

.. math::

    h_{k+1}^t & = \sum_i \sigma(z_i^t)(1 - \sigma(z_i^t)) \\
    & - \sum_i y_i \bigg\{ \frac{\sigma(z_i^t) (1 - \sigma(z_i^t))}{q(z_i^t)} - \frac{\sigma(z_i^t)}{q(z_i^t)^2} \bigg\}


If :math:`k > 0`,

.. math::

    \begin{eqnarray}
    h_{k+1}^t & = \sum_i \sigma(z_i^t)(1 - \sigma(z_i^t)) x_{i,k+1}^2 \\
    & - \sum_i y_i \bigg\{ \frac{\sigma(z_i^t) (1 - \sigma(z_i^t))}{q(z_i^t)}
    & - \frac{\sigma(z_i^t)}{q(z_i^t)^2} \bigg\}x_{i,k+1}^2 + \lambda(1-\alpha)
    \end{eqnarray}

.. code-block:: python

    def hess_loss_k(z, alpha, rl, xk, y, k):
        """Hessian update for a single coordinate
        """
        q = qu(z)
        s = expit(z)
        grad_s = s*(1-s)
        grad_s_by_q = grad_s/q - s/(q*q)
        if(k == 0):
            hk = np.sum(grad_s) - np.sum(y*grad_s_by_q)
        else:
            hk = np.sum(grad_s*xk*xk) - np.sum(y*grad_s_by_q*xk*xk) + rl*(1-alpha)
        return hk


Regularization paths and warm restarts
--------------------------------------

We often find the optimal regularization parameter :math:`\lambda` through cross-validation.
Thus, in practice, we fit the model several times over a range of :math:`\lambda`'s
:math:`\{ \lambda_{max} \geq \dots \geq \lambda_0\}`.

Instead of re-fitting the model each time, we can solve the problem for the
most-regularized model (:math:`\lambda_{max}`) and then initialize the subsequent
model with this solution. The path that each parameter takes through the range of
regularization parameters is known as the regularization path, and the trick of
initializing each model with the previous model's solution is known as a warm restart.

In practice, this significantly speeds up convergence.


Implementation
--------------

The optimization step is implemented in ``fit`` method in ``GLM``. We will add
pseudo code on how algorithm works soon.
